proof/refine/AARCH64/ArchCSpace_R.thy
@@ -549,23 +549,6 @@ lemma create_reply_master_corres[CSpace_R_2_assms]:
   apply (clarsimp simp: valid_pspace'_def cte_wp_at'_def)
   done
 
-lemma cte_map_nat_to_cref:
-  "\<lbrakk> n < 2 ^ b; b < word_bits \<rbrakk> \<Longrightarrow>
-   cte_map (p, nat_to_cref b n) = p + (of_nat n * 2^cte_level_bits)"
-  apply (clarsimp simp: cte_map_def nat_to_cref_def shiftl_t2n
-                 dest!: less_is_drop_replicate)
-  apply (subst mult_ac)
-  apply (rule arg_cong [where f="\<lambda>x. x * 2^cte_level_bits"])
-  apply (subst of_drop_to_bl)
-  apply (simp add: word_bits_def)
-  apply (subst mask_eq_iff_w2p)
-   apply (simp add: word_size)
-  apply (simp add: word_less_nat_alt word_size word_bits_def)
-  apply (rule order_le_less_trans; assumption?)
-  apply (subst unat_of_nat)
-  apply (rule mod_less_eq_dividend)
-  done
-
 declare azobj_refs'_only_vcpu[simp]
 
 lemma setupReplyMaster_global_refs[wp]:
